added files

theories/LogicalRelation/Definition/Bool.v
@@ -1,6 +1,6 @@
 (** * LogRel.LogicalRelation.Definition.Bool : Definition of the logical relation for bool *)
 From Stdlib Require Import CRelationClasses.
-From LogRel Require Import Utils Syntax.All GenericTyping.
+From LogRel Require Import Utils Syntax.All GenericTyping Monad.
 From LogRel.LogicalRelation.Definition Require Import Prelude Ne.
 
 Set Primitive Projections.
@@ -11,7 +11,7 @@ Set Polymorphic Inductive Cumulativity.
 (** ** Reducibility of boolean type *)
 Module BoolRedTy.
 
-  Record BoolRedTy `{ta : tag} `{WfType ta} `{RedType ta}
+  Record SBoolRedTy `{ta : tag} `{WfType ta} `{RedType ta}
     {Γ : context} {A B : term}
   : Set :=
   {
@@ -19,26 +19,30 @@ Module BoolRedTy.
     redR : [Γ |- B :⤳*: tBool]
   }.
 
-  Arguments BoolRedTy {_ _ _}.
+  Arguments SBoolRedTy {_ _ _}.
+
+  Definition BoolRedTy `{ta : tag} `{WfType ta} `{RedType ta} Γ A B : Type :=
+    Split (fun Δ (ρ : Δ ≤ Γ) => SBoolRedTy Δ A⟨ρ⟩ B⟨ρ⟩).
 
   Section BoolRedTy.
   Context `{ta : tag} `{WfType ta} `{RedType ta}.
 
-  Definition whredL {Γ A B} : BoolRedTy Γ A B -> [Γ |- A ↘].
+  Definition whredL {Γ A B} : SBoolRedTy Γ A B -> [Γ |- A ↘].
   Proof. intros []; econstructor; tea; constructor. Defined.
 
-  Definition whredR {Γ A B} : BoolRedTy Γ A B -> [Γ |- B ↘].
+  Definition whredR {Γ A B} : SBoolRedTy Γ A B -> [Γ |- B ↘].
   Proof. intros []; econstructor; tea; constructor. Defined.
 
   End BoolRedTy.
 
 End BoolRedTy.
 
-Export BoolRedTy(BoolRedTy, Build_BoolRedTy).
+Export BoolRedTy(SBoolRedTy, BoolRedTy, Build_SBoolRedTy).
+Notation "[ Γ ||-SBool A ≅ B ]" := (BoolRedTy Γ A B) (at level 0, Γ, A at level 50).
 Notation "[ Γ ||-Bool A ≅ B ]" := (BoolRedTy Γ A B) (at level 0, Γ, A at level 50).
 
 #[program]
-Instance WhRedTyBoolRedTy `{GenericTypingProperties} {Γ} : WhRedTyRel Γ (BoolRedTy Γ) :=
+Instance WhRedTyBoolRedTy `{GenericTypingProperties} {Γ} : WhRedTyRel Γ (SBoolRedTy Γ) :=
   {|
     whredtyL := fun A B RAB => BoolRedTy.whredL RAB ;
     whredtyR := fun A B RAB => BoolRedTy.whredR RAB ;
@@ -50,49 +54,52 @@ Module BoolRedTmEq.
 Section BoolRedTmEq.
   Context `{ta : tag} `{WfContext ta} `{WfType ta} `{ConvType ta}
     `{RedType ta} `{Typing ta} `{ConvNeuConv ta} `{ConvTerm ta}
-    `{RedTerm ta} {Γ : context}.
+    `{RedTerm ta}.
 
-  Inductive BoolPropEq : term -> term -> Set :=
+  Inductive BoolPropEq Γ : term -> term -> Set :=
   | trueReq :
-    BoolPropEq tTrue tTrue
+    BoolPropEq Γ tTrue tTrue
   | falseReq :
-    BoolPropEq tFalse tFalse
-  | neReq {ne ne'} : [Γ ||-NeNf ne ≅ ne' : tBool] -> BoolPropEq ne ne'.
+    BoolPropEq Γ tFalse tFalse
+  | neReq {ne ne'} : [Γ ||-NeNf ne ≅ ne' : tBool] -> BoolPropEq Γ ne ne'.
 
 
-  Record BoolRedTmEq {t u} : Set :=
+  Record SBoolRedTmEq {Γ t u} : Set :=
     {
       nfL : term ;
       nfR : term ;
       redL : [Γ |- t :⤳*: nfL : tBool] ;
       redR : [Γ |- u :⤳*: nfR : tBool ] ;
       eq : [Γ |- nfL ≅ nfR : tBool] ;
-      prop : BoolPropEq nfL nfR
+      prop : BoolPropEq Γ nfL nfR
   }.
-  Arguments BoolRedTmEq : clear implicits.
+  Arguments SBoolRedTmEq : clear implicits.
+
+  Definition BoolRedTmEq Γ t u : Set :=
+    Split (fun Δ (ρ : Δ ≤ Γ) => SBoolRedTmEq Δ t⟨ρ⟩ u⟨ρ⟩).
 
   Section Def.
     Context `{!GenericTypingProperties _ _ _ _ _ _ _ _ _}.
 
-    Lemma BoolPropEq_isBool {t t' : term} :
-      BoolPropEq t t' -> isBool t × isBool t'.
+    Lemma BoolPropEq_isBool Γ {t t' : term} :
+      BoolPropEq Γ t t' -> isBool t × isBool t'.
     Proof.
       intros [| |?? []]; split; constructor.
       all: eapply convneu_whne; eassumption + now symmetry.
     Defined.
 
-    Definition whnfL {t u} : BoolPropEq t u -> whnf t.
+    Definition whnfL {Γ t u} : BoolPropEq Γ t u -> whnf t.
     Proof. intros []%BoolPropEq_isBool; now eapply isBool_whnf. Qed.
 
-    Definition whnfR {t u} : BoolPropEq t u -> whnf u.
+    Definition whnfR {Γ t u} : BoolPropEq Γ t u -> whnf u.
     Proof. intros []%BoolPropEq_isBool; now eapply isBool_whnf. Qed.
 
-    Definition whredL {t u} : BoolRedTmEq t u -> [Γ |- t ↘ tBool].
+    Definition whredL {Γ t u} : SBoolRedTmEq Γ t u -> [Γ |- t ↘ tBool].
     Proof.
       intros []; econstructor; tea; now eapply whnfL.
     Defined.
 
-    Definition whredR {t u} : BoolRedTmEq t u -> [Γ |- u ↘ tBool].
+    Definition whredR {Γ t u} : SBoolRedTmEq Γ t u -> [Γ |- u ↘ tBool].
     Proof.
       intros []; econstructor; tea; now eapply whnfR.
     Defined.
@@ -102,15 +109,17 @@ Section BoolRedTmEq.
 
 End BoolRedTmEq.
 Arguments BoolPropEq {_ _ _}.
+Arguments SBoolRedTmEq {_ _ _ _ _}.
 Arguments BoolRedTmEq {_ _ _ _ _}.
 End BoolRedTmEq.
 
-Export BoolRedTmEq(BoolRedTmEq,Build_BoolRedTmEq,BoolPropEq,BoolPropEq_isBool).
+Export BoolRedTmEq(BoolRedTmEq,SBoolRedTmEq,Build_SBoolRedTmEq,BoolPropEq,BoolPropEq_isBool).
 
+Notation "[ Γ ||-SBool t ≅ u :Bool]" := (@SBoolRedTmEq _ _ _ _ _ _ _ Γ t u).
 Notation "[ Γ ||-Bool t ≅ u :Bool]" := (@BoolRedTmEq _ _ _ _ _ _ _ Γ t u).  (* (at level 0, Γ, t, u at level 50). *)
 
 #[program]
-Instance BoolRedTmEqWhRed `{GenericTypingProperties} {Γ} : WhRedTmRel Γ tBool (BoolRedTmEq Γ) :=
+Instance BoolRedTmEqWhRed `{GenericTypingProperties} {Γ} : WhRedTmRel Γ tBool (SBoolRedTmEq Γ) :=
   {| whredtmL := fun t u Rtu => BoolRedTmEq.whredL Rtu ;
     whredtmR := fun t u Rtu => BoolRedTmEq.whredR Rtu |}.
 Next Obligation.
