theories/LogicalRelation/Definition/Empty.v
@@ -1,6 +1,6 @@
 (** * LogRel.LogicalRelation.Definition.Empty : Definition of the logical relation for the empty type *)
 From Stdlib Require Import CRelationClasses.
-From LogRel Require Import Utils Syntax.All GenericTyping.
+From LogRel Require Import Utils Syntax.All GenericTyping Monad.
 From LogRel.LogicalRelation.Definition Require Import Prelude Ne.
 
 Set Primitive Projections.
@@ -10,7 +10,7 @@ Set Polymorphic Inductive Cumulativity.
 (** ** Reducibility of empty type *)
 Module EmptyRedTy.
 
-  Record EmptyRedTy `{ta : tag} `{WfType ta} `{RedType ta}
+  Record SEmptyRedTy `{ta : tag} `{WfType ta} `{RedType ta}
     {Γ : context} {A B : term}
   : Set :=
   {
@@ -18,24 +18,29 @@ Module EmptyRedTy.
     redR : [Γ |- B :⤳*: tEmpty]
   }.
 
-  Arguments EmptyRedTy {_ _ _}.
+  Arguments SEmptyRedTy {_ _ _}.
+
+  Definition EmptyRedTy `{ta : tag} `{WfType ta} `{RedType ta} Γ A B : Set :=
+    Split (fun Δ (ρ : Δ ≤ Γ) => SEmptyRedTy Δ A⟨ρ⟩ B⟨ρ⟩).
+
   Section EmptyRedTy.
   Context `{ta : tag} `{WfType ta} `{RedType ta}.
 
-  Definition whredL {Γ A B} : EmptyRedTy Γ A B -> [Γ |- A ↘].
+  Definition whredL {Γ A B} : SEmptyRedTy Γ A B -> [Γ |- A ↘].
   Proof. intros []; econstructor; tea; constructor. Defined.
 
-  Definition whredR {Γ A B} : EmptyRedTy Γ A B -> [Γ |- B ↘].
+  Definition whredR {Γ A B} : SEmptyRedTy Γ A B -> [Γ |- B ↘].
   Proof. intros []; econstructor; tea; constructor. Defined.
 
   End EmptyRedTy.
 End EmptyRedTy.
 
-Export EmptyRedTy(EmptyRedTy, Build_EmptyRedTy).
+Export EmptyRedTy(EmptyRedTy, SEmptyRedTy, Build_SEmptyRedTy).
+Notation "[ Γ ||-SEmpty A ≅ B ]" := (SEmptyRedTy Γ A B) (at level 0, Γ, A at level 50).
 Notation "[ Γ ||-Empty A ≅ B ]" := (EmptyRedTy Γ A B) (at level 0, Γ, A at level 50).
 
 #[program]
-Instance WhRedTyEmptyRedTy `{GenericTypingProperties} {Γ} : WhRedTyRel Γ (EmptyRedTy Γ) :=
+Instance WhRedTyEmptyRedTy `{GenericTypingProperties} {Γ} : WhRedTyRel Γ (SEmptyRedTy Γ) :=
   {|
     whredtyL := fun A B RAB => EmptyRedTy.whredL RAB ;
     whredtyR := fun A B RAB => EmptyRedTy.whredR RAB ;
@@ -49,7 +54,7 @@ Section EmptyRedTmEq.
     `{RedType ta} `{Typing ta} `{ConvNeuConv ta} `{ConvTerm ta}
     `{RedTerm ta}.
 
-  Record EmptyRedTmEq {Γ t u} : Set :=
+  Record SEmptyRedTmEq {Γ t u} : Set :=
     {
       nfL : term ;
       nfR : term ;
@@ -57,31 +62,37 @@ Section EmptyRedTmEq.
       redR : [Γ |- u :⤳*: nfR : tEmpty ] ;
       eq : [Γ ||-NeNf nfL ≅ nfR : tEmpty]
   }.
-  Arguments  EmptyRedTmEq : clear implicits.
+  Arguments  SEmptyRedTmEq : clear implicits.
+
+  Definition EmptyRedTmEq Γ t u : Set :=
+    Split (fun Δ (ρ : Δ ≤ Γ) => SEmptyRedTmEq Δ t⟨ρ⟩ u⟨ρ⟩).
+
   Section Def.
     Context `{!GenericTypingProperties _ _ _ _ _ _ _ _ _}.
 
-    Definition whredL {Γ t u} : EmptyRedTmEq Γ t u -> [Γ |- t ↘ tEmpty].
+    Definition whredL {Γ t u} : SEmptyRedTmEq Γ t u -> [Γ |- t ↘ tEmpty].
     Proof.
       intros []; econstructor; tea; unshelve eapply NeNf.whredL; cycle 3; tea.
     Defined.
 
-    Definition whredR {Γ t u} : EmptyRedTmEq Γ t u -> [Γ |- u ↘ tEmpty].
+    Definition whredR {Γ t u} : SEmptyRedTmEq Γ t u -> [Γ |- u ↘ tEmpty].
     Proof.
       intros []; econstructor; tea; unshelve eapply NeNf.whredR; cycle 3; tea.
     Defined.
   End  Def.
 
 End EmptyRedTmEq.
+Arguments SEmptyRedTmEq {_ _ _ _}.
 Arguments EmptyRedTmEq {_ _ _ _}.
 End EmptyRedTmEq.
 
-Export EmptyRedTmEq(EmptyRedTmEq,Build_EmptyRedTmEq).
+Export EmptyRedTmEq(EmptyRedTmEq, SEmptyRedTmEq, Build_SEmptyRedTmEq).
 
-Notation "[ Γ ||-Empty t ≅ u :Empty]" := (@EmptyRedTmEq _ _ _ _ _ _ _ Γ t u).  (* (at level 0, Γ, t, u at level 50). *)
+Notation "[ Γ ||-Empty t ≅ u :Empty]" := (@EmptyRedTmEq _ _ _ _ _ _ _ Γ t u).
+Notation "[ Γ ||-SEmpty t ≅ u :Empty]" := (@SEmptyRedTmEq _ _ _ _ _ _ _ Γ t u).  (* (at level 0, Γ, t, u at level 50). *)
 
 #[program]
-Instance EmptyRedTmEqWhRed `{GenericTypingProperties} {Γ} : WhRedTmRel Γ tEmpty (EmptyRedTmEq Γ) :=
+Instance EmptyRedTmEqWhRed `{GenericTypingProperties} {Γ} : WhRedTmRel Γ tEmpty (SEmptyRedTmEq Γ) :=
   {| whredtmL := fun t u Rtu => EmptyRedTmEq.whredL Rtu ;
     whredtmR := fun t u Rtu => EmptyRedTmEq.whredR Rtu |}.
 Next Obligation.
