theories/Monad.v
@@ -1,0 +1,218 @@
+From LogRel Require Import Utils Syntax.All.
+
+Inductive DTree (L : Fcontext) : Set :=
+  | leaf : DTree L
+  | node (new : newnat L):
+    DTree (Fcons' L new true) ->
+    DTree (Fcons' L new false) ->
+    DTree L.
+
+
+Arguments node {_ _}.
+
+Fixpoint overtree {L} (d : DTree L) L' : SProp :=
+  match d with
+  | leaf _ => L' ≤ε L
+  | @node _ new dt df =>
+    match decide_in L' new with
+    | is_in true _ => overtree dt L'
+    | is_in false _ => overtree df L'
+    | is_notin _ => SFalse
+    end
+  end.
+
+Lemma overtree_Fwk {L L'} {d : DTree L} : overtree d L' -> L' ≤ε L.
+Proof.
+  induction d as [ | L new Lt iht Lf ihf] ; cbn ; intros H ; auto.
+  destruct (decide_in L' new).
+  - eapply Fwk_compose.
+    destruct b.
+    + now apply iht.
+    + now apply ihf.
+    + eapply Fwk_Fstep; apply Fwk_id. 
+  - destruct H.
+Qed.
+
+
+Fixpoint DTree_psh {L} L' {Fρ : L' ≤ε L} : DTree L -> DTree L'.
+Proof.
+  intros d.
+  destruct d as [| new dt df].
+  - apply leaf.
+  - destruct (decide_in L' new) as [b hin |hnotin].
+    + refine (DTree_psh (Fcons' L new b) L' _ (match b with true=>dt|false=>df end)).
+      now eapply Fwk_new.
+    + refine (@node _ (Build_newnat L' new hnotin) _ _).
+      * unshelve eapply (DTree_psh _ _ _ dt).
+        now eapply Fwk_Fup.
+      * unshelve eapply (DTree_psh _ _ _ df).
+        now eapply Fwk_Fup.
+Defined.
+
+Lemma overtree_psh (L L' L'' : Fcontext) (Fρ : L' ≤ε L) (d : DTree L) :
+  overtree (DTree_psh L' d) L'' -> overtree d L''.
+Proof.
+  intros Hover; assert (Fρ' : L'' ≤ε L') by now eapply overtree_Fwk.
+  revert L' L'' Fρ Fρ' Hover;
+  induction d as [ | L new dt iht df ihf];
+  intros * Fρ' Hover; cbn in *.
+  - now eapply Fwk_compose.
+  - destruct (decide_in L' new) as [[] hin'|hnotin']; cbn in *;
+    destruct (decide_in L'' new) as [[] hin''|hnotin''].
+    1,5,9: easy.
+    2,4: eauto using notin_is_not_in.
+    + destruct (functionality_inversion _ new (Fρ' _ _ hin') hin'').
+    + destruct (functionality_inversion _ new hin'' (Fρ' _ _ hin')).
+    + refine (iht _ _ _ _ Hover).
+      now eapply (Fwk_new (Build_newnat L' new hnotin') true Fρ').
+    + refine (ihf _ _ _ _ Hover).
+      now eapply (Fwk_new (Build_newnat L' new hnotin') false Fρ').
+Qed.
+
+Local Set Universe Polymorphism.
+
+Definition psh@{i j} Γ : Type@{j} := forall Δ, Δ ≤ Γ -> Type@{i}.
+
+Definition psh_psh {Γ Δ} (ρ : Γ ≤ Δ): psh Δ -> psh Γ :=
+  fun A Ξ σ => A Ξ (σ ∘w ρ).
+
+Lemma psh_rew {Γ} (A : psh Γ) : forall Δ (ρ ρ' : Δ ≤ Γ), ρ =1 ρ' -> A Δ ρ -> A Δ ρ'.
+Proof.
+  intros Δ ρ ρ' heq1 hA.
+  apply wk_to_ren_inj in heq1.
+  now destruct heq1.
+Qed.
+
+Definition hom {Γ} (A B : psh Γ) := forall Δ ρ, A Δ ρ -> B Δ ρ.
+
+Lemma hom_psh {Γ} {A B : psh Γ} : hom A B -> forall Δ (ρ : Δ ≤ Γ), hom (psh_psh ρ A) (psh_psh ρ B).
+Proof.
+  intros hhom Δ ρ Ξ σ hA.
+  apply hhom.
+  apply hA.
+Qed.
+
+Record Split@{i j} {Γ} (A : psh@{i j} Γ) : Type@{i} := {
+  dtree : DTree Γ;
+  cover : forall (Δ : context) ρ, overtree dtree Δ -> A Δ ρ
+}.
+
+Definition Split_psh {Γ} : psh Γ -> psh Γ:=
+ fun A Δ ρ => Split (psh_psh ρ A).
+
+Lemma split_hom_psh Γ (A B : psh Γ) : hom A B -> Split A -> Split B.
+Proof.
+  intros hhom hA.
+  destruct hA as [dA hA].
+  exists dA.
+  intros Δ ρ hover.
+  apply hhom.
+  now apply hA.
+Qed.
+
+Lemma Split_wkn Γ (A : psh Γ) : Split A -> forall Δ ρ, Split_psh A Δ ρ.
+Proof.
+  intros [dA hA] Δ ρ.
+  exists (DTree_psh Δ dA).
+  intros Ξ σ Hover.
+  apply hA.
+  now eapply overtree_psh.
+Qed.
+
+Lemma Split_wkn_inv Γ A : (forall Δ (ρ : Δ ≤ Γ), Split_psh A Δ ρ) -> Split A.
+Proof.
+  intros.
+  eapply split_hom_psh.
+  2: apply (X Γ wk_id).
+  intros Δ ρ hA.
+  refine (psh_rew A _ _ _ _ hA).
+  bsimpl.
+  reflexivity.
+Qed.
+
+Definition shf {Γ} (A : psh Γ) := forall Δ (ρ : Δ ≤ Γ) new,
+    A (Δ,,new↦true) (wk_Fstep _ _ ρ) ->
+    A (Δ,,new↦false) (wk_Fstep _ _ ρ) ->
+    A Δ ρ.
+
+Lemma shf_psh {Γ A} : shf A -> forall Δ (ρ : Δ ≤ Γ), shf (psh_psh ρ A).
+Proof.
+  intros hAshf Δ ρ Ξ σ new hAt hAf.
+  unfold psh_psh, shf in *.
+  now eapply hAshf.
+Qed.
+
+Lemma Split_shf {Γ} {A : psh Γ} : shf (Split_psh A).
+Proof.
+  intros Δ ρ new [dAt hAt] [dAf hAf].
+  exists (node dAt dAf).
+  intros Ξ σ hover.
+  cbn in hover.
+  destruct (decide_in Ξ new) as [[] hin|hnotin].
+  - specialize (hAt Ξ (wk_new new true σ hin) hover).
+    refine (psh_rew A _ _ _ _ hAt).
+    bsimpl. reflexivity.
+  - specialize (hAf Ξ (wk_new new false σ hin) hover).
+    refine (psh_rew A _ _ _ _ hAf).
+    bsimpl. reflexivity.
+  - destruct hover.
+Qed.
+
+
+Lemma split_bind_alg : forall Γ (A B: psh Γ),
+  shf B ->
+  hom A B ->
+  Split A -> (forall Δ (ρ : Δ ≤ Γ), B Δ ρ).
+Proof.
+  intros [Γ L] A B hBshf hhom [dA hA]; cbn in *.
+  induction dA as [L |L new dt ihAt df ihAf].
+  - intros Δ ρ. cbn in *.
+    apply hhom.
+    apply hA.
+    apply ρ.
+  - change L with (Fctx (Build_context Γ L)) in new.
+    specialize (ihAt (psh_psh (wk_Fstep new true wk_id) A)
+      (psh_psh (wk_Fstep new true wk_id) B) (shf_psh hBshf _ _) (hom_psh hhom _ _)).
+    specialize (ihAf (psh_psh (wk_Fstep new false wk_id) A)
+      (psh_psh (wk_Fstep new false wk_id) B) (shf_psh hBshf _ _) (hom_psh hhom _ _)).
+    assert (forall (b: bool) Δ (ρ : Δ ≤ (Build_context Γ L),,new ↦ b),
+      overtree (match b with true => dt| false => df end) Δ -> psh_psh (wk_Fstep new b wk_id) A Δ ρ) as H.
+    1:{ intros b Δ ρ hover.
+        apply hA; cbn.
+        rewrite (decide_in_in Δ new b (Fwk ρ new b (in_hereF L new b))).
+        now destruct b. }
+    specialize (ihAt (H true)).
+    specialize (ihAf (H false)).
+    clear H.
+    intros Δ ρ.
+    destruct (decide_in Δ new) as [[] hin|hnotin].
+    + specialize (ihAt Δ (wk_new new true ρ hin)).
+      refine (psh_rew B _ _ ρ _ ihAt).
+      bsimpl. reflexivity.
+    + specialize (ihAf Δ (wk_new new false ρ hin)).
+      refine (psh_rew B _ _ ρ _ ihAf).
+      bsimpl. reflexivity.
+    + set (new' := Build_newnat Δ new hnotin).
+      eapply hBshf.
+      * specialize (ihAt (Δ,, new' ↦ true) (wk_Fup _ _ true new ρ new new')).
+        refine (psh_rew B _ _ _ _ ihAt).
+        bsimpl. reflexivity.
+      * specialize (ihAf (Δ,, new' ↦ false) (wk_Fup _ _ false new ρ new new')).
+        refine (psh_rew B _ _ _ _ ihAf).
+        bsimpl. reflexivity.
+Qed.
+
+
+
+Lemma Split_bind : forall Γ (A B : psh Γ),
+  Split A ->
+  (forall Δ (ρ : Δ ≤ Γ), A Δ ρ -> Split_psh B Δ ρ) ->
+  Split B.
+Proof.
+  intros Γ A B hA f.
+  apply Split_wkn_inv.
+  apply (split_bind_alg Γ A).
+  - apply Split_shf.
+  - exact f.
+  - apply hA.
+Qed.
