theories/Syntax/Computations.v
@@ -1,0 +1,58 @@
+From Stdlib Require Import ssreflect Morphisms Setoid.
+From LogRel Require Import Utils BasicAst AutoSubst.Extra.
+
+Set Primitive Projections.
+
+Fixpoint nat_to_term n : term :=
+  match n with
+  | 0 => tZero
+  | S n => tSucc (nat_to_term n)
+  end.
+
+Fixpoint nSucc n t : term :=
+  match n with
+  | 0 => t
+  | S n => tSucc (nSucc n t)
+  end.
+
+Definition bool_to_term b : term :=
+  match b with
+  | true => tTrue
+  | false => tFalse
+  end.
+
+Lemma bool_to_term_ren : forall b ρ, (bool_to_term b)⟨ρ⟩ = bool_to_term b.
+Proof.
+  intros [|] ρ; reflexivity.
+Qed.
+
+Lemma nat_to_term_ren : forall n ρ, (nat_to_term n)⟨ρ⟩ = nat_to_term n.
+Proof.
+  intros n ρ.
+  induction n; cbn.
+  - reflexivity.
+  - now f_equal.
+Qed.
+
+Lemma nSucc_ren : forall n t ρ, (nSucc n t)⟨ρ⟩ = nSucc n (t⟨ρ⟩).
+Proof.
+  intros n t ρ.
+  induction n; cbn.
+  - reflexivity.
+  - now f_equal.
+Qed.
+
+Lemma nat_to_term_inj n n' : nat_to_term n = nat_to_term n' -> n = n'.
+Proof.
+  revert n'.
+  induction n.
+  - intros n' e.
+    destruct n'.
+    + reflexivity.
+    + inversion e.
+  - intros [|] e.
+    + inversion e.
+    + inversion e; subst.
+      f_equal.
+      now apply IHn.
+Qed.
